Removed remaining smt calls

Adaptive_State_Counting/FSM/FSM3.thy
@@ -34,7 +34,7 @@ fun is_wf_transition :: "('state, 'b) FSM_scheme \<Rightarrow> 'state Transition
 fun wf_transitions :: "('state, 'b) FSM_scheme \<Rightarrow> 'state Transition list" where
   "wf_transitions M = filter (is_wf_transition M) (transitions M)"
 
-abbreviation "h M \<equiv> set (wf_transitions M)"
+abbreviation(input) "h M \<equiv> set (wf_transitions M)"
 
 
 
@@ -834,7 +834,7 @@ proof
                         and "path B q2 p2"
                         and "io = p_io p1" 
                         and "io = p_io p2"
-      using product_path[of A B q1 q2] by auto
+      using product_path[of A B q1 q2 p] by auto
     then show "io \<in> LS A q1 \<inter> LS B q2" 
       unfolding LS.simps by blast
   qed
@@ -1344,13 +1344,11 @@ proof
   let ?p1 = "left_path p"
   let ?p2 = "right_path p"
 
-  have "path A (initial A) ?p1"
-  and  "path B (initial B) ?p2"
-    using product_path[of A B "initial A" "initial B" p]
-    using \<open>path (product A B) (initial (product A B)) p\<close> by auto 
+  have "path A (initial A) ?p1 \<and> path B (initial B) ?p2"
+    by (metis \<open>path (product A B) (initial (product A B)) p\<close> product_path[of A B "initial A" "initial B" p] product_simps(1))
 
   moreover have "target p (initial (product A B)) = (target ?p1 (initial A), target ?p2 (initial B))"
-    by (induction p; auto)  
+    by (induction p; force)  
 
   ultimately show "q \<in> (nodes A) \<times> (nodes B)"
     by (metis (no_types, lifting) SigmaI \<open>q = target p (initial (product A B))\<close> nodes_path_initial)
@@ -4361,7 +4359,7 @@ value "language_up_to_length M_ex 5"
 
 
 
-fun calculate_preamble_set_naive :: "('a, 'b) FSM_scheme \<Rightarrow> 'a \<Rightarrow> (Input \<times> Output) list set option" where
+definition calculate_preamble_set_naive :: "('a, 'b) FSM_scheme \<Rightarrow> 'a \<Rightarrow> (Input \<times> Output) list set option" where
   "calculate_preamble_set_naive M q = (let n = size M - 1 in
     (case 
       (filter 
@@ -4381,13 +4379,13 @@ proof -
                 (\<lambda> S . language_up_to_length S (Suc ( size M - 1 )) = language_up_to_length S ( size M - 1 ) \<and>  is_preamble_set M q (set (language_up_to_length S ( size M - 1 )))) 
                 (generate_submachines M))
               ) ( size M - 1 ))"
-    using assms unfolding calculate_preamble_set_naive.simps
+    using assms unfolding calculate_preamble_set_naive_def
     by (metis (no_types, lifting) hd_Cons_tl list.case_eq_if option.discI option.inject)
 
   have *: "filter 
         (\<lambda> S . language_up_to_length S (Suc ( size M - 1 )) = language_up_to_length S ( size M - 1 ) \<and>  is_preamble_set M q (set (language_up_to_length S ( size M - 1 )))) 
         (generate_submachines M) \<noteq> []"
-    by (metis (mono_tags, lifting) assms calculate_preamble_set_naive.simps list.case_eq_if option.discI)
+    by (metis (mono_tags, lifting) assms calculate_preamble_set_naive_def list.case_eq_if option.discI)
 
   let ?S = "hd (filter 
         (\<lambda> S . language_up_to_length S (Suc ( size M - 1 )) = language_up_to_length S ( size M - 1 ) \<and>  is_preamble_set M q (set (language_up_to_length S ( size M - 1 )))) 
@@ -4486,7 +4484,7 @@ proof -
     using \<open>S \<in> set (generate_submachines M)\<close> filter_empty_conv[of ?f "generate_submachines M"] by blast
 
   then show "calculate_preamble_set_naive M q \<noteq> None"
-    unfolding calculate_preamble_set_naive.simps
+    unfolding calculate_preamble_set_naive_def
     by (metis (mono_tags, lifting) list.case_eq_if option.distinct(1))   
 qed
 
@@ -4640,10 +4638,8 @@ definition canonical_separator :: "('a,'b) FSM_scheme \<Rightarrow> 'a \<Rightar
 value[code] "(canonical_separator M_ex 2 3)"
 value[code] "trim_transitions (canonical_separator M_ex 2 3)"
 
-fun is_Inl :: "'a + 'b \<Rightarrow> bool" where
-  "is_Inl (Inl x) = True" |
-  "is_Inl (Inr x) = False"
-fun is_state_separator_from_canonical_separator :: "(('a \<times> 'a) + 'a,'b) FSM_scheme \<Rightarrow> 'a \<Rightarrow> 'a \<Rightarrow> (('a \<times> 'a) + 'a,'b) FSM_scheme \<Rightarrow> bool" where
+
+definition is_state_separator_from_canonical_separator :: "(('a \<times> 'a) + 'a,'b) FSM_scheme \<Rightarrow> 'a \<Rightarrow> 'a \<Rightarrow> (('a \<times> 'a) + 'a,'b) FSM_scheme \<Rightarrow> bool" where
   "is_state_separator_from_canonical_separator CSep q1 q2 S = (
     is_submachine S CSep 
     \<and> single_input S
@@ -4652,7 +4648,7 @@ fun is_state_separator_from_canonical_separator :: "(('a \<times> 'a) + 'a,'b) F
     \<and> deadlock_state S (Inr q2)
     \<and> ((Inr q1) \<in> nodes S)
     \<and> ((Inr q2) \<in> nodes S)
-    \<and> (\<forall> q \<in> nodes S . (q \<noteq> Inr q1 \<and> q \<noteq> Inr q2) \<longrightarrow> (is_Inl q \<and> \<not> deadlock_state S q))
+    \<and> (\<forall> q \<in> nodes S . (q \<noteq> Inr q1 \<and> q \<noteq> Inr q2) \<longrightarrow> (isl q \<and> \<not> deadlock_state S q))
     \<and> (\<forall> q \<in> nodes S . \<forall> x \<in> set (inputs CSep) . (\<exists> t \<in> h S . t_source t = q \<and> t_input t = x) \<longrightarrow> (\<forall> t' \<in> h CSep . t_source t' = q \<and> t_input t' = x \<longrightarrow> t' \<in> h S))
 )"
 
@@ -4662,7 +4658,7 @@ fun generate_choices :: "('a \<times> ('b list)) list \<Rightarrow> ('a \<times>
   "generate_choices (xys#xyss) = concat (map (\<lambda> xy' . map (\<lambda> xys' . xy' # xys') (generate_choices xyss)) ((fst xys, None) # (map (\<lambda> y . (fst xys, Some y)) (snd xys))))"
 
 value "generate_choices [(0::nat,[0::nat,1,2])]"
-value "generate_choices [(0::nat,[0::nat,1,2]),(1,[10,20,30])]"
+value "generate_choices [(0::nat,[0::nat,1]),(1,[10,20])]"
 
 lemma concat_map_hd_tl_elem: 
   assumes "hd cs \<in> set P1"
@@ -4684,13 +4680,33 @@ proof (induction xyss arbitrary: cs xys)
   case Nil
   have "(cs \<in> set (generate_choices [xys])) = (cs \<in> set ([(fst xys, None)] # map (\<lambda>y. [(fst xys, Some y)]) (snd xys)))" 
     unfolding generate_choices.simps by auto
+  moreover have "(cs \<in> set ([(fst xys, None)] # map (\<lambda>y. [(fst xys, Some y)]) (snd xys))) \<Longrightarrow> (length cs = length [xys] \<and>
+     fst (hd cs) = fst xys \<and>
+     (snd (hd cs) = None \<or> snd (hd cs) \<noteq> None \<and> the (snd (hd cs)) \<in> set (snd xys)) \<and>
+     tl cs \<in> set (generate_choices []))"
+    by auto
   moreover have "(length cs = length [xys] \<and>
      fst (hd cs) = fst xys \<and>
      (snd (hd cs) = None \<or> snd (hd cs) \<noteq> None \<and> the (snd (hd cs)) \<in> set (snd xys)) \<and>
-     tl cs \<in> set (generate_choices [])) = (cs \<in> set ([(fst xys, None)] # map (\<lambda>y. [(fst xys, Some y)]) (snd xys)))"
-    (* TODO: smt *)
-    by (smt Suc_length_conv fst_conv generate_choices.simps(1) imageE image_eqI length_0_conv list.sel(1) list.sel(3) list.set_intros(1) list.set_sel(2) list.size(4) option.collapse option.sel prod.collapse set_ConsD set_map snd_conv tl_Nil)
-    
+     tl cs \<in> set (generate_choices [])) \<Longrightarrow> (cs \<in> set ([(fst xys, None)] # map (\<lambda>y. [(fst xys, Some y)]) (snd xys)))"
+    unfolding generate_choices.simps(1)
+  proof -
+    assume a1: "length cs = length [xys] \<and> fst (hd cs) = fst xys \<and> (snd (hd cs) = None \<or> snd (hd cs) \<noteq> None \<and> the (snd (hd cs)) \<in> set (snd xys)) \<and> tl cs \<in> set [[]]"
+    have f2: "\<forall>ps. ps = [] \<or> ps = (hd ps::'a \<times> 'b option) # tl ps"
+      by (meson list.exhaust_sel)
+    have f3: "cs \<noteq> []"
+      using a1 by fastforce
+    have "snd (hd cs) = None \<longrightarrow> (fst xys, None) = hd cs"
+      using a1 by (metis prod.exhaust_sel)
+    moreover
+    { assume "hd cs # tl cs \<noteq> [(fst xys, Some (the (snd (hd cs))))]"
+      then have "snd (hd cs) = None"
+        using a1 by (metis (no_types) length_0_conv length_tl list.sel(3) option.collapse prod.exhaust_sel) }
+    ultimately have "cs \<in> insert [(fst xys, None)] ((\<lambda>b. [(fst xys, Some b)]) ` set (snd xys))"
+      using f3 f2 a1 by fastforce
+    then show ?thesis
+      by simp
+  qed 
   ultimately show ?case by blast
 next
   case (Cons a xyss)
@@ -4725,6 +4741,63 @@ next
   ultimately show ?case by blast
 qed 
 
+lemma list_append_idx_prop : 
+  "(\<forall> i . (i < length xs \<longrightarrow> P (xs ! i))) = (\<forall> j . ((j < length (ys@xs) \<and> j \<ge> length ys) \<longrightarrow> P ((ys@xs) ! j)))"
+proof -
+  have "\<And> j . \<forall>i<length xs. P (xs ! i) \<Longrightarrow> j < length (ys @ xs) \<Longrightarrow> length ys \<le> j \<longrightarrow> P ((ys @ xs) ! j)"
+    by (simp add: nth_append)
+  moreover have "\<And> i . (\<forall> j . ((j < length (ys@xs) \<and> j \<ge> length ys) \<longrightarrow> P ((ys@xs) ! j))) \<Longrightarrow> i < length xs \<Longrightarrow> P (xs ! i)"
+  proof -
+    fix i assume "(\<forall> j . ((j < length (ys@xs) \<and> j \<ge> length ys) \<longrightarrow> P ((ys@xs) ! j)))" and "i < length xs"
+    then have "P ((ys@xs) ! (length ys + i))"
+      by (metis add_strict_left_mono le_add1 length_append)
+    moreover have "P (xs ! i) = P ((ys@xs) ! (length ys + i))"
+      by simp
+    ultimately show "P (xs ! i)" by blast
+  qed
+  ultimately show ?thesis by blast
+qed
+
+lemma list_append_idx_prop2 : 
+  assumes "length xs' = length xs"
+      and "length ys' = length ys"
+  shows "(\<forall> i . (i < length xs \<longrightarrow> P (xs ! i) (xs' ! i))) = (\<forall> j . ((j < length (ys@xs) \<and> j \<ge> length ys) \<longrightarrow> P ((ys@xs) ! j) ((ys'@xs') ! j)))"
+proof -
+
+  have "\<forall>i<length xs. P (xs ! i) (xs' ! i) \<Longrightarrow>
+    \<forall>j. j < length (ys @ xs) \<and> length ys \<le> j \<longrightarrow> P ((ys @ xs) ! j) ((ys' @ xs') ! j)"
+    using assms
+  proof -
+    assume a1: "\<forall>i<length xs. P (xs ! i) (xs' ! i)"
+    { fix nn :: nat
+      have ff1: "\<forall>n na. (na::nat) + n - n = na"
+        by simp
+      have ff2: "\<forall>n na. (na::nat) \<le> n + na"
+        by auto
+      then have ff3: "\<forall>as n. (ys' @ as) ! n = as ! (n - length ys) \<or> \<not> length ys \<le> n"
+        using ff1 by (metis (no_types) add.commute assms(2) eq_diff_iff nth_append_length_plus)
+      have ff4: "\<forall>n bs bsa. ((bsa @ bs) ! n::'b) = bs ! (n - length bsa) \<or> \<not> length bsa \<le> n"
+        using ff2 ff1 by (metis (no_types) add.commute eq_diff_iff nth_append_length_plus)
+      have "\<forall>n na nb. ((n::nat) + nb \<le> na \<or> \<not> n \<le> na - nb) \<or> \<not> nb \<le> na"
+        using ff2 ff1 by (metis le_diff_iff)
+      then have "(\<not> nn < length (ys @ xs) \<or> \<not> length ys \<le> nn) \<or> P ((ys @ xs) ! nn) ((ys' @ xs') ! nn)"
+        using ff4 ff3 a1 by (metis add.commute length_append not_le) }
+    then show ?thesis
+      by blast
+  qed
+
+  moreover have "(\<forall>j. j < length (ys @ xs) \<and> length ys \<le> j \<longrightarrow> P ((ys @ xs) ! j) ((ys' @ xs') ! j)) \<Longrightarrow>\<forall>i<length xs. P (xs ! i) (xs' ! i)"
+    using assms
+    by (metis le_add1 length_append nat_add_left_cancel_less nth_append_length_plus) 
+
+  ultimately show ?thesis by blast
+qed
+    
+
+  
+
+
+
 
 lemma generate_choices_idx : "cs \<in> set (generate_choices xyss) = (length cs = length xyss \<and> (\<forall> i < length cs . (fst (cs ! i)) = (fst (xyss ! i)) \<and> ((snd (cs ! i)) = None \<or> ((snd (cs ! i)) \<noteq> None \<and> the (snd (cs ! i)) \<in> set (snd (xyss ! i))))))"
 proof (induction xyss arbitrary: cs)
@@ -4734,21 +4807,6 @@ next
   case (Cons xys xyss)
 
 
-  have "(\<forall>i<length (tl cs).
-                    fst (tl cs ! i) = fst (xyss ! i) \<and>
-                    (snd (tl cs ! i) = None \<or> snd (tl cs ! i) \<noteq> None \<and> the (snd (tl cs ! i)) \<in> set (snd (xyss ! i))))
-              = (\<forall>i<length (tl cs).
-                    fst (cs ! (Suc i)) = fst ((xys#xyss) ! (Suc i)) \<and>
-                    (snd (cs ! (Suc i)) = None \<or> snd (cs ! (Suc i)) \<noteq> None \<and> the (snd (cs ! (Suc i))) \<in> set (snd ((xys#xyss) ! (Suc i)))))" 
-    using nth_tl by fastforce
-  then have *: "(\<forall>i<length (tl cs).
-                    fst (tl cs ! i) = fst (xyss ! i) \<and>
-                    (snd (tl cs ! i) = None \<or> snd (tl cs ! i) \<noteq> None \<and> the (snd (tl cs ! i)) \<in> set (snd (xyss ! i))))
-               = (\<forall>i<length cs. i > 0 \<longrightarrow>
-                    (fst (cs ! i) = fst ((xys#xyss) ! i) \<and>
-                      (snd (cs ! i) = None \<or> snd (cs ! i) \<noteq> None \<and> the (snd (cs ! i)) \<in> set (snd ((xys#xyss) ! i)))))"
-    (* TODO: smt *)
-    by (smt Nitpick.size_list_simp(2) Suc_lessD Suc_mono Suc_pred less_SucE tl_Nil zero_less_Suc)
 
   have "cs \<in> set (generate_choices (xys#xyss)) = (length cs = length (xys#xyss) \<and> fst (hd cs) = fst xys \<and> ((snd (hd cs) = None \<or> (snd (hd cs) \<noteq> None \<and> the (snd (hd cs)) \<in> set (snd xys)))) \<and> (tl cs \<in> set (generate_choices xyss)))"
     using generate_choices_hd_tl by metis
@@ -4762,7 +4820,7 @@ next
           fst (tl cs ! i) = fst (xyss ! i) \<and>
           (snd (tl cs ! i) = None \<or> snd (tl cs ! i) \<noteq> None \<and> the (snd (tl cs ! i)) \<in> set (snd (xyss ! i))))))"
     using Cons.IH[of "tl cs"] by blast
-  then have "cs \<in> set (generate_choices (xys#xyss)) 
+  then have *: "cs \<in> set (generate_choices (xys#xyss)) 
     = (length cs = length (xys#xyss) 
       \<and> fst (hd cs) = fst xys 
       \<and> ((snd (hd cs) = None \<or> (snd (hd cs) \<noteq> None \<and> the (snd (hd cs)) \<in> set (snd xys)))) 
@@ -4771,27 +4829,47 @@ next
           (snd (tl cs ! i) = None \<or> snd (tl cs ! i) \<noteq> None \<and> the (snd (tl cs ! i)) \<in> set (snd (xyss ! i)))))"
     by auto
 
-  moreover have "length cs = length (xys#xyss) \<Longrightarrow> (fst (hd cs) = fst xys \<and> ((snd (hd cs) = None \<or> (snd (hd cs) \<noteq> None \<and> the (snd (hd cs)) \<in> set (snd xys))))) = 
-          (fst (cs ! 0) = fst ((xys#xyss) ! 0) \<and> (snd (cs ! 0) = None \<or> snd (cs ! 0) \<noteq> None \<and> the (snd (cs ! 0)) \<in> set (snd ((xys#xyss) ! 0))))"
-    by (metis hd_conv_nth length_greater_0_conv list.simps(3) nth_Cons_0)
-    
-  ultimately have "cs \<in> set (generate_choices (xys#xyss)) 
-    = (length cs = length (xys#xyss)  
-      \<and> (fst (cs ! 0) = fst ((xys#xyss) ! 0) \<and> (snd (cs ! 0) = None \<or> snd (cs ! 0) \<noteq> None \<and> the (snd (cs ! 0)) \<in> set (snd ((xys#xyss) ! 0))))
-      \<and> (\<forall>i<length cs. i > 0 \<longrightarrow>
-                    (fst (cs ! i) = fst ((xys#xyss) ! i) \<and>
-                      (snd (cs ! i) = None \<or> snd (cs ! i) \<noteq> None \<and> the (snd (cs ! i)) \<in> set (snd ((xys#xyss) ! i))))))"  
-    using * by blast
 
-  moreover have "length cs = length (xys#xyss) \<Longrightarrow> ((fst (cs ! 0) = fst ((xys#xyss) ! 0) \<and> (snd (cs ! 0) = None \<or> snd (cs ! 0) \<noteq> None \<and> the (snd (cs ! 0)) \<in> set (snd ((xys#xyss) ! 0))))
-        \<and> (\<forall>i<length cs. i > 0 \<longrightarrow>
-                      (fst (cs ! i) = fst ((xys#xyss) ! i) \<and>
-                        (snd (cs ! i) = None \<or> snd (cs ! i) \<noteq> None \<and> the (snd (cs ! i)) \<in> set (snd ((xys#xyss) ! i))))))
-      = (\<forall>i<length cs.
-           fst (cs ! i) = fst ((xys # xyss) ! i) \<and>
-           (snd (cs ! i) = None \<or>
-            snd (cs ! i) \<noteq> None \<and> the (snd (cs ! i)) \<in> set (snd ((xys # xyss) ! i))))" 
-    by fastforce
+  have "cs \<in> set (generate_choices (xys#xyss)) \<Longrightarrow> (length cs = length (xys # xyss) \<and>
+                    (\<forall>i<length cs.
+                        fst (cs ! i) = fst ((xys # xyss) ! i) \<and>
+                        (snd (cs ! i) = None \<or>
+                        snd (cs ! i) \<noteq> None \<and> the (snd (cs ! i)) \<in> set (snd ((xys # xyss) ! i)))))"
+  proof -
+    assume "cs \<in> set (generate_choices (xys#xyss))"
+    then have p1: "length cs = length (xys#xyss)"
+          and p2: "fst (hd cs) = fst xys "
+          and p3: "((snd (hd cs) = None \<or> (snd (hd cs) \<noteq> None \<and> the (snd (hd cs)) \<in> set (snd xys))))"
+          and p4: "(\<forall>i<length (tl cs).
+                  fst (tl cs ! i) = fst (xyss ! i) \<and>
+                  (snd (tl cs ! i) = None \<or> snd (tl cs ! i) \<noteq> None \<and> the (snd (tl cs ! i)) \<in> set (snd (xyss ! i))))"
+      using * by blast+
+    then have "length xyss = length (tl cs)" and "length (xys # xyss) = length ([hd cs] @ tl cs)"
+      by auto
+    
+    have "[hd cs]@(tl cs) = cs"
+      by (metis (no_types) p1 append.left_neutral append_Cons length_greater_0_conv list.collapse list.simps(3)) 
+    then have p4b: "(\<forall>i<length cs. i > 0 \<longrightarrow>
+                    (fst (cs ! i) = fst ((xys#xyss) ! i) \<and>
+                      (snd (cs ! i) = None \<or> snd (cs ! i) \<noteq> None \<and> the (snd (cs ! i)) \<in> set (snd ((xys#xyss) ! i)))))"
+      using p4 list_append_idx_prop2[of xyss "tl cs" "xys#xyss" "[hd cs]@(tl cs)" "\<lambda> x y . fst x = fst y \<and>
+                    (snd x = None \<or> snd x \<noteq> None \<and> the (snd x) \<in> set (snd y))", OF \<open>length xyss = length (tl cs)\<close> \<open>length (xys # xyss) = length ([hd cs] @ tl cs)\<close>]
+      by (metis (no_types, lifting) One_nat_def Suc_pred \<open>length (xys # xyss) = length ([hd cs] @ tl cs)\<close> \<open>length xyss = length (tl cs)\<close> length_Cons list.size(3) not_less_eq nth_Cons_pos nth_append) 
+
+    have p4a :"(fst (cs ! 0) = fst ((xys#xyss) ! 0) \<and> (snd (cs ! 0) = None \<or> snd (cs ! 0) \<noteq> None \<and> the (snd (cs ! 0)) \<in> set (snd ((xys#xyss) ! 0))))"
+      using p1 p2 p3 by (metis hd_conv_nth length_greater_0_conv list.simps(3) nth_Cons_0)
+
+    show ?thesis using p1 p4a p4b by fastforce
+  qed
+
+
+  moreover have "(length cs = length (xys # xyss) \<and>
+                    (\<forall>i<length cs.
+                        fst (cs ! i) = fst ((xys # xyss) ! i) \<and>
+                        (snd (cs ! i) = None \<or>
+                        snd (cs ! i) \<noteq> None \<and> the (snd (cs ! i)) \<in> set (snd ((xys # xyss) ! i))))) \<Longrightarrow> cs \<in> set (generate_choices (xys#xyss))"
+    using * 
+    by (metis (no_types, lifting) Nitpick.size_list_simp(2) Suc_mono hd_conv_nth length_greater_0_conv length_tl list.sel(3) list.simps(3) nth_Cons_0 nth_tl) 
 
   ultimately show ?case by blast
 qed
@@ -4879,7 +4957,7 @@ proof -
     deadlock_state (trim_transitions S) (Inr q2) \<and>
     Inr q1 \<in> nodes (trim_transitions S) \<and>
     Inr q2 \<in> nodes (trim_transitions S)"
-    using assms unfolding is_state_separator_from_canonical_separator.simps  
+    using assms unfolding is_state_separator_from_canonical_separator_def
     using trim_transitions_submachine[of S CSep]
     using trim_transitions_single_input[of S]
     using trim_transitions_acyclic[of S]
@@ -4887,15 +4965,15 @@ proof -
     using trim_transitions_nodes[of S] 
     by blast
 
-  have "(\<forall>q\<in>nodes S. q \<noteq> Inr q1 \<and> q \<noteq> Inr q2 \<longrightarrow> is_Inl q \<and> \<not> deadlock_state S q)"
-    using assms unfolding is_state_separator_from_canonical_separator.simps by blast
-  then have p2: "(\<forall>q\<in>nodes (trim_transitions S). q \<noteq> Inr q1 \<and> q \<noteq> Inr q2 \<longrightarrow> is_Inl q \<and> \<not> deadlock_state (trim_transitions S) q)"
+  have "(\<forall>q\<in>nodes S. q \<noteq> Inr q1 \<and> q \<noteq> Inr q2 \<longrightarrow> isl q \<and> \<not> deadlock_state S q)"
+    using assms unfolding is_state_separator_from_canonical_separator_def by blast
+  then have p2: "(\<forall>q\<in>nodes (trim_transitions S). q \<noteq> Inr q1 \<and> q \<noteq> Inr q2 \<longrightarrow> isl q \<and> \<not> deadlock_state (trim_transitions S) q)"
     using trim_transitions_nodes[of S]  trim_transitions_deadlock_state_nodes[of _ S] by blast
 
   have *: "(\<forall>q\<in>nodes S.
       \<forall>x\<in>set (inputs CSep).
          (\<exists>t\<in>h S. t_source t = q \<and> t_input t = x) \<longrightarrow> (\<forall>t'\<in>h CSep. t_source t' = q \<and> t_input t' = x \<longrightarrow> t' \<in> h S))"
-    using assms unfolding is_state_separator_from_canonical_separator.simps by blast
+    using assms unfolding is_state_separator_from_canonical_separator_def by blast
   have p3: "\<And> q x . q\<in>nodes (trim_transitions S) \<Longrightarrow> x\<in>set (inputs CSep) \<Longrightarrow>
            (\<exists>t\<in>h (trim_transitions S). t_source t = q \<and> t_input t = x) \<Longrightarrow>
            (\<forall>t'\<in>h CSep. t_source t' = q \<and> t_input t' = x \<longrightarrow> t' \<in> h (trim_transitions S))"
@@ -4922,7 +5000,7 @@ proof -
     then show "(\<forall>t'\<in>h CSep. t_source t' = q \<and> t_input t' = x \<longrightarrow> t' \<in> h (trim_transitions S))" by blast
   qed
 
-  from p1 p2 p3 show ?thesis unfolding  is_state_separator_from_canonical_separator.simps by blast
+  from p1 p2 p3 show ?thesis unfolding is_state_separator_from_canonical_separator_def by blast
 qed
 
 lemma transitions_reorder :  
@@ -4967,12 +5045,12 @@ proof -
         and "deadlock_state S (Inr q2)"
         and "Inr q1 \<in> nodes S"
         and "Inr q2 \<in> nodes S"
-        and "(\<forall>q\<in>nodes S. q \<noteq> Inr q1 \<and> q \<noteq> Inr q2 \<longrightarrow> is_Inl q \<and> \<not> deadlock_state S q)"
+        and "(\<forall>q\<in>nodes S. q \<noteq> Inr q1 \<and> q \<noteq> Inr q2 \<longrightarrow> isl q \<and> \<not> deadlock_state S q)"
         and "(\<forall>q\<in>nodes S.
               \<forall>x\<in>set (inputs CSep).
                  (\<exists>t\<in>h S. t_source t = q \<and> t_input t = x) \<longrightarrow>
                  (\<forall>t'\<in>h CSep. t_source t' = q \<and> t_input t' = x \<longrightarrow> t' \<in> h S))"
-    using assms(1) unfolding is_state_separator_from_canonical_separator.simps by linarith+
+    using assms(1) unfolding is_state_separator_from_canonical_separator_def by linarith+
 
   note transitions_reorder[OF assms(2-5)]
 
@@ -4988,8 +5066,8 @@ proof -
     using \<open>deadlock_state S (Inr q2)\<close> \<open>h S' = h S\<close> unfolding deadlock_state.simps by blast
   moreover have "Inr q1 \<in> nodes S'" and "Inr q2 \<in> nodes S'"
     using \<open>Inr q1 \<in> nodes S\<close> \<open>Inr q2 \<in> nodes S\<close> \<open>nodes S' = nodes S\<close> by blast+
-  moreover have "(\<forall>q\<in>nodes S'. q \<noteq> Inr q1 \<and> q \<noteq> Inr q2 \<longrightarrow> is_Inl q \<and> \<not> deadlock_state S' q)"
-    using \<open>(\<forall>q\<in>nodes S. q \<noteq> Inr q1 \<and> q \<noteq> Inr q2 \<longrightarrow> is_Inl q \<and> \<not> deadlock_state S q)\<close> \<open>nodes S' = nodes S\<close> \<open>h S' = h S\<close> unfolding deadlock_state.simps by blast
+  moreover have "(\<forall>q\<in>nodes S'. q \<noteq> Inr q1 \<and> q \<noteq> Inr q2 \<longrightarrow> isl q \<and> \<not> deadlock_state S' q)"
+    using \<open>(\<forall>q\<in>nodes S. q \<noteq> Inr q1 \<and> q \<noteq> Inr q2 \<longrightarrow> isl q \<and> \<not> deadlock_state S q)\<close> \<open>nodes S' = nodes S\<close> \<open>h S' = h S\<close> unfolding deadlock_state.simps by blast
   moreover have "(\<forall>q\<in>nodes S'.
               \<forall>x\<in>set (inputs CSep).
                  (\<exists>t\<in>h S'. t_source t = q \<and> t_input t = x) \<longrightarrow>
@@ -4999,7 +5077,7 @@ proof -
                  (\<exists>t\<in>h S. t_source t = q \<and> t_input t = x) \<longrightarrow>
                  (\<forall>t'\<in>h CSep. t_source t' = q \<and> t_input t' = x \<longrightarrow> t' \<in> h S))\<close> 
           \<open>h S' = h S\<close> \<open>nodes S' = nodes S\<close> by blast
-  ultimately show ?thesis unfolding is_state_separator_from_canonical_separator.simps by linarith
+  ultimately show ?thesis unfolding is_state_separator_from_canonical_separator_def by linarith
 qed
 
 lemma generate_submachine_for_contained_assn: "assn \<in> set assns \<Longrightarrow> generate_submachine_from_assignment CSep assn \<in> set (map (\<lambda> assn . generate_submachine_from_assignment CSep assn) assns)"
@@ -5036,18 +5114,12 @@ proof -
         and "deadlock_state ?S (Inr q2)"
         and "Inr q1 \<in> nodes ?S"
         and "Inr q2 \<in> nodes ?S"
-        and "(\<forall>q\<in>nodes ?S. q \<noteq> Inr q1 \<and> q \<noteq> Inr q2 \<longrightarrow> is_Inl q \<and> \<not> deadlock_state ?S q)"
+        and "(\<forall>q\<in>nodes ?S. q \<noteq> Inr q1 \<and> q \<noteq> Inr q2 \<longrightarrow> isl q \<and> \<not> deadlock_state ?S q)"
         and "(\<forall>q\<in>nodes ?S.
               \<forall>x\<in>set (inputs ?CSep).
                  (\<exists>t\<in>h ?S. t_source t = q \<and> t_input t = x) \<longrightarrow>
                  (\<forall>t'\<in>h ?CSep. t_source t' = q \<and> t_input t' = x \<longrightarrow> t' \<in> h ?S))"
-    unfolding is_state_separator_from_canonical_separator.simps by linarith+
-
-  let ?ncs = "nodes_from_distinct_paths ?CSep"
-  let ?ns = "nodes_from_distinct_paths ?S"
-
-  let ?cbc = "map (\<lambda>q. (q, filter (\<lambda>x. \<exists>t\<in>h ?CSep. t_source t = q \<and> t_input t = x) (inputs ?CSep)))"
-  let ?cbs = "map (\<lambda>q. (q, filter (\<lambda>x. \<exists>t\<in>h ?S. t_source t = q \<and> t_input t = x) (inputs ?S)))"
+    unfolding is_state_separator_from_canonical_separator_def by linarith+
 
   have "finite (nodes ?S)"
     by (simp add: nodes_finite) 
